change defs to typed

docs/formalization/ismodel/CoreCps.thy
@@ -4,6 +4,7 @@ begin
 
 
 
+
 datatype  typeexpr = AnyTp
      |
       ConstTp
@@ -15,15 +16,23 @@ datatype  typeexpr = AnyTp
       ErrorTp
 
 
+(* TODO: use typeclasse s*)
+fun isCorrectTp :: "typeexpr \<Rightarrow> bool" where
+  "isCorrectTp AnyTp = True"
+ |"isCorrectTp ConstTp = True"
+ |"isCorrectTp (ArrowTp t1 t2) = ((isCorrectTp t1)\<and>(isCorrectTp t2))"
+ |"isCorrectTp (MonadTp t) = isCorrectTp t"
+ |"isCorrectTp ErrorTp = False"
+
+
+
 
 datatype expr = ConstantExpr int
   |
    Let int typeexpr expr expr
   |
-   Ref int typeexpr
+   Ref int typeexpr 
   |
-   Block "expr list" 
- |
    If expr expr expr
   |
    While expr expr 
@@ -36,15 +45,14 @@ datatype expr = ConstantExpr int
  |
    MflatMap expr expr
  |
+   Await expr
+ |
    ExternalFun int typeexpr
  |
    Error string
 
 
 
-fun isError :: "expr \<Rightarrow> bool" where
-   "isError (Error s) = True" |
-   "isError other = False"
 
 fun lub :: "typeexpr \<Rightarrow> typeexpr \<Rightarrow> typeexpr" where
    "lub ConstTp ConstTp = ConstTp"
@@ -73,7 +81,6 @@ type_synonym varIndex = int
 type_synonym typeVarState = "varIndex \<Rightarrow> typeexpr"
 
 
-
 fun typeExpr :: "expr \<Rightarrow> typeVarState \<Rightarrow> typeexpr" where
     "typeExpr (ConstantExpr x) s = ConstTp"
   |
@@ -81,15 +88,11 @@ fun typeExpr :: "expr \<Rightarrow> typeVarState \<Rightarrow> typeexpr" where
   |
     "typeExpr (Ref i it) s = (if (it = s(i)) then it else ErrorTp)"
   |
-    "typeExpr (Block l) s = (case l of
-                               [] \<Rightarrow> ConstTp
-                              |
-                               x # [] \<Rightarrow>  (typeExpr x s)
-                              |
-                               h # t \<Rightarrow> (typeExpr (Block t) s)
-                            )"
-  |
-    "typeExpr (If cond ifTrue ifFalse) s = (lub (typeExpr ifTrue s) (typeExpr ifFalse s))"
+    "typeExpr (If cond ifTrue ifFalse) s = (
+        case (typeExpr cond s) of
+          ConstTp \<Rightarrow> (lub (typeExpr ifTrue s) (typeExpr ifFalse s))
+          | other \<Rightarrow> ErrorTp 
+    )"
   |
     "typeExpr (While e1 e2) s = ConstTp"
   |
@@ -97,13 +100,18 @@ fun typeExpr :: "expr \<Rightarrow> typeVarState \<Rightarrow> typeexpr" where
   |
     "typeExpr (App x arg) s =
                 (case (typeExpr x s) of
+                     ErrorTp \<Rightarrow> ErrorTp
+                    |
                      (ArrowTp xi xo) \<Rightarrow> if ((typeExpr arg s) = xi) then xo else ErrorTp
                     |
                      other \<Rightarrow> ErrorTp
                 )  
     "
   |
-    "typeExpr (Mpure x) s = MonadTp (typeExpr x s)"
+    "typeExpr (Mpure x) s = ( case (typeExpr x s) of 
+                                 ErrorTp \<Rightarrow> ErrorTp
+                               | tx \<Rightarrow> MonadTp tx
+                            )"
   |
     "typeExpr (MflatMap fa f) s = (
         case (typeExpr fa s) of
@@ -113,11 +121,53 @@ fun typeExpr :: "expr \<Rightarrow> typeVarState \<Rightarrow> typeexpr" where
           | other \<Rightarrow> ErrorTp
     )"
   |
+    "typeExpr (Await e) s = (
+       case (typeExpr e s) of
+         MonadTp te \<Rightarrow> te
+        | other     \<Rightarrow> ErrorTp
+    )"
+  |
     "typeExpr (ExternalFun fi ft) s = ft"
   | 
     "typeExpr (Error e) s = ErrorTp"
+  
+
 
 datatype AsyncKind = AKSync | AKAsync AsyncKind | AKLambda AsyncKind | AKError
+
+fun isCorrectAk :: "AsyncKind \<Rightarrow> bool" where
+   " isCorrectAk AKSync = True "
+ | " isCorrectAk (AKAsync k) = (isCorrectAk k) "
+ | " isCorrectAk (AKLambda k) = (isCorrectAk k)"
+ | " isCorrectAk AKError = False "
+
+fun isCompatibleAk :: "AsyncKind \<Rightarrow> AsyncKind \<Rightarrow> bool" where
+   "isCompatibleAk AKSync AKSync = True"
+ |
+   "isCompatibleAk AKSync (AKAsync k2) = isCompatibleAk AKSync k2"
+ |
+   "isCompatibleAk AKSync (AKLambda k2) = False"
+ |
+   "isCompatibleAk AKSync AKError = False"
+ |
+   "isCompatibleAk (AKAsync k1) AKSync = isCompatibleAk k1 AKSync"
+ |
+   "isCompatibleAk (AKAsync k1) (AKAsync k2) = isCompatibleAk k1 k2"
+ |
+   "isCompatibleAk (AKAsync k1) (AKLambda k2) = False"
+ |
+   "isCompatibleAk (AKAsync k1) AKError = False"
+ |
+   "isCompatibleAk (AKLambda k1) AKSync = False"
+ |
+   "isCompatibleAk (AKLambda k1) (AKAsync k2) = False"
+ |
+   "isCompatibleAk (AKLambda k1) (AKLambda k2) = isCompatibleAk k1 k2"
+ |
+   "isCompatibleAk AKError x = False"
+ |
+   "isCompatibleAk x  AKError = False"
+
 
 datatype CpsTree =
         CpsTreePure expr
@@ -128,17 +178,56 @@ datatype CpsTree =
         |
         CpsTreeLambda int typeexpr CpsTree
         |
+         (* analog of SeqCpsTree *)
+        CpsTreeLet int typeexpr expr CpsTree 
+        |
         ErrorCpsTree
 
+fun typeCpsTree:: "CpsTree \<Rightarrow> typeVarState \<Rightarrow> typeexpr" where
+       "typeCpsTree (CpsTreePure expr) s = MonadTp (typeExpr expr s)"
+     |
+       "typeCpsTree (CpsTreeFlatMap src i tb fbody) s = (
+          case (typeCpsTree src s) of
+            MonadTp srct \<Rightarrow> 
+                (case (typeCpsTree fbody (s(i:=srct))) of
+                    ArrowTp fx fy \<Rightarrow> if (fx = srct) then fy else ErrorTp
+                   | other \<Rightarrow> ErrorTp)
+          |other \<Rightarrow> ErrorTp
+       )"
+     |
+       "typeCpsTree (CpsTreeAsync e k) s = (
+           (typeExpr e s) 
+       )"
+     |
+       "typeCpsTree (CpsTreeLambda v vt body) s = (
+         case (typeCpsTree body (s(v:=vt))) of
+            ErrorTp \<Rightarrow> ErrorTp
+           | rt     \<Rightarrow> ArrowTp vt rt
+       )"
+     |
+       "typeCpsTree (CpsTreeLet v vt init body) s = (
+          if (vt = ErrorTp) then ErrorTp else typeCpsTree body (s(v:=vt)) 
+       )"
+     |
+       "typeCpsTree ErrorCpsTree s = ErrorTp" 
+
+
+fun isCorrectExpr::"expr \<Rightarrow> typeVarState \<Rightarrow> bool" where
+       "isCorrectExpr e s = ((typeExpr e s) \<noteq> ErrorTp)" 
+
+fun isCorrectCps :: "CpsTree \<Rightarrow> typeVarState \<Rightarrow> bool" where
+   "isCorrectCps t s = ((typeCpsTree t s) \<noteq> ErrorTp)"
+ 
 
 fun asyncKind :: "CpsTree \<Rightarrow> AsyncKind" where
     "asyncKind (CpsTreePure e) = AKSync"
   |
-    "asyncKind (CpsTreeAsync e k) = k"
+    "asyncKind (CpsTreeAsync e k) = AKAsync k"
   |
     "asyncKind (CpsTreeFlatMap source i tp fbody) = (
        case (asyncKind source) of
-           (AKAsync Sync) \<Rightarrow> (asyncKind fbody)
+            (AKSync) \<Rightarrow> AKAsync (asyncKind fbody)
+          | (AKAsync Sync) \<Rightarrow> AKAsync (asyncKind fbody) 
           | other \<Rightarrow> AKError
     )"
   |
@@ -149,26 +238,42 @@ fun asyncKind :: "CpsTree \<Rightarrow> AsyncKind" where
     *)
     "asyncKind (CpsTreeLambda i tp body) = AKLambda (asyncKind body)"
   |
+    "asyncKind (CpsTreeLet v vt vv cpsBody) = asyncKind cpsBody"
+  |
     "asyncKind ErrorCpsTree = AKError"
-      
+    
+definition isRedusableCps::"CpsTree \<Rightarrow> typeVarState \<Rightarrow> bool" where
+   "isRedusableCps t s \<longleftrightarrow> (isCorrectCps t s) \<and> ((asyncKind t) \<noteq> AKError)"
+
+
 (*
  analog of CpsTree.transformed
 *)
-fun cpsTreeToExpr :: "CpsTree \<Rightarrow> expr" where 
-   "cpsTreeToExpr (CpsTreePure e) = Mpure e"
+fun cpsTreeToExpr :: "CpsTree \<Rightarrow> typeVarState \<Rightarrow> expr" where 
+   "cpsTreeToExpr (CpsTreePure e) s = Mpure e"
  |
-   "cpsTreeToExpr (CpsTreeFlatMap arg v vt vbody) = 
-                                MflatMap (cpsTreeToExpr arg) (Lambda v vt (cpsTreeToExpr vbody))"
+   "cpsTreeToExpr (CpsTreeFlatMap arg v vt vbody) s = 
+                   MflatMap (cpsTreeToExpr arg s) (Lambda v vt (cpsTreeToExpr vbody (s(v:=vt))))"
  |
-   "cpsTreeToExpr (CpsTreeAsync e k) = (
+   "cpsTreeToExpr (CpsTreeAsync e k) s = (
        case k of
            AKSync \<Rightarrow> e
+         | AKAsync k1 \<Rightarrow> (
+             case (typeExpr e s) of
+                 (MonadTp et) \<Rightarrow> if (isCorrectTp et) then 
+                                    (MflatMap e (Lambda 1 et (Ref 1 et)))
+                                 else (Error ''AAA'')
+                 |other \<Rightarrow> Error ''Invalud async kind''
+           )
          | other \<Rightarrow> Error ''Invalid async kind''
    )"   (* TODO: handle AsynK*(Sync)  *)
  |
-   "cpsTreeToExpr (CpsTreeLambda v vt vbody) = (Lambda v vt (cpsTreeToExpr vbody))"
+   "cpsTreeToExpr (CpsTreeLambda v vt vbody) s = (Lambda v vt (cpsTreeToExpr vbody (s(v:=vt))))"
+ |
+   "cpsTreeToExpr (CpsTreeLet v vt vv cpsBody) s = (Let v vt vv (cpsTreeToExpr cpsBody (s(v:=vt))))"
   |
-   "cpsTreeToExpr ErrorCpsTree = Error ''ErrorCpsTree'' "
+   "cpsTreeToExpr ErrorCpsTree s = Error ''ErrorCpsTree'' "
+ 
 
 
 fun unpureCpsTree :: "CpsTree \<Rightarrow> (expr option)" where
@@ -195,25 +300,96 @@ fun unpureCpsTree :: "CpsTree \<Rightarrow> (expr option)" where
          None \<Rightarrow> None
    )"
  |
+  "unpureCpsTree (CpsTreeLet v vt vv cpsBody) = (
+      case (unpureCpsTree cpsBody) of
+        Some body \<Rightarrow> Some (Let v vt (vv) (body))
+        |
+        None \<Rightarrow> None 
+  )"
+ |
   "unpureCpsTree ErrorCpsTree = None" 
+
+lemma correctNotError: "isCorrectCps (t::CpsTree) s \<Longrightarrow> t \<noteq> ErrorCpsTree"
+  by auto
+
+lemma correctNoErrorKind: "(isCorrectCps (t::CpsTree) (s::typeVarState)) \<Longrightarrow> (asyncKind t) \<noteq> AKError"
+  (*nitpick*)
+  
+  oops
+  
+
+
+
+lemma letUnputAsBody: " 
+    (isCorrectTp (vt::typeexpr))
+    \<and>(isCorrectExpr (vv::expr) (s::typeVarState))
+    \<and>(isCorrectCps (cpsBody::CpsTree) s)
+    \<and>((unpureCpsTree cpsBody) \<noteq> None) \<Longrightarrow>
+        (unpureCpsTree (CpsTreeLet (v::int) vt vv cpsBody)) \<noteq> None"
+  (*nitpick *)
+  apply auto
+  done
+
+lemma flatMapUnputAsBody: "
+   (isCorrectCps (source::CpsTree) (s::typeVarState))
+   \<and>
+   ((unpureCpsTree source) \<noteq> None)
+   \<and>
+   (isCorrectTp (vt::typeexpr))
+   \<and>
+   (isCorrectCps (fbody::CpsTree) s)
+   \<and>
+   ((unpureCpsTree fbody) \<noteq> None)
+           \<Longrightarrow>
+           unpureCpsTree((CpsTreeFlatMap source v vt fbody) ) \<noteq> None
+"
+  apply auto
+  done
+
+lemma syncHaveUnpure: "(isCorrectCps (t::CpsTree) (s::typeVarState) )\<and>(asyncKind(t) = AKSync) \<Longrightarrow> unpureCpsTree(t) \<noteq> None"
+  nitpick
+  apply(induct t)
+  apply auto
+  apply (smt (verit, del_insts) AsyncKind.distinct(1) AsyncKind.simps(15) AsyncKind.simps(16) AsyncKind.simps(17) AsyncKind.simps(18) isCorrectAk.cases)
+  sorry
+
 
 (*
  CpsTransform 
 *)
-fun exprToCpsTree :: "expr \<Rightarrow> CpsTree" where
-    "exprToCpsTree (ConstantExpr c) =  CpsTreePure (ConstantExpr c)"
+fun exprToCpsTree :: "expr \<Rightarrow> typeVarState \<Rightarrow> CpsTree" where
+    "exprToCpsTree (ConstantExpr c) s =  CpsTreePure (ConstantExpr c)"
   |
-    "exprToCpsTree (Let v vt vv body) = (
-        let cpsv = exprToCpsTree vv in
-         let cpsbody = exprToCpsTree body in
-           case (asyncKind cpsv) of 
-              AKSync \<Rightarrow>
-                case (asyncKind cpsbody) of
-                   AKSync \<Rightarrow>
-                       CpsTreePure (Let v vt (unpureCpsTree vv) (unpureCpsTree cpsbody))
+    "exprToCpsTree (Ref i tp) s = CpsTreePure (Ref i tp)"
+  |
+    "exprToCpsTree (Let v vt vv body) s = (
+        let cpsv = (exprToCpsTree vv s) in (
+         let cpsbody = (exprToCpsTree body s) in
+           (case (unpureCpsTree cpsv) of
+             Some pureV \<Rightarrow> 
+               (case (unpureCpsTree cpsbody) of
+                   Some pureBody \<Rightarrow> CpsTreePure (Let v vt (pureV) (pureBody))
+                  |None \<Rightarrow> CpsTreeLet v vt (pureV) cpsbody
+               )
+             |None \<Rightarrow>
+                (case (asyncKind cpsv) of
+                    AKAsync ik \<Rightarrow> 
+                     (CpsTreeFlatMap (cpsv) v vt (cpsbody))
+                    | AKLambda bk \<Rightarrow> ErrorCpsTree
+                )
+           )
+        )
     )"
+  |
+   (* TODO *)
+   "exprToCpsTree (If c e1 e2) s = (
+    let cpsC = (exprToCpsTree c s); 
+        cpsE1 = (exprToCpsTree e1 s);
+        cpsE2 = (exprToCpsTree e2 s) in (
+       ErrorCpsTree 
+    )
+   )"
     
     
-
 
 end
